PrimParser.lean
@@ -1,7 +1,7 @@
 import PrimParser.Basic
 import PrimParser.Char
 import PrimParser.GradedMonad
+import PrimParser.Input
 import PrimParser.Necessity
 import PrimParser.NonEmptyList
 import PrimParser.Properties
-import PrimParser.Text
